DynamoDbEncryption/dafny/StructuredEncryption/src/AwsCryptographyDbEncryptionSdkStructuredEncryptionOperations.dfy
@@ -141,7 +141,8 @@ module AwsCryptographyDbEncryptionSdkStructuredEncryptionOperations refines Abst
   } by method {
     reveal SumValueSize();
     var sum : uint64 := 0;
-    for i := |fields| downto 0
+    SequenceIsSafeBecauseItIsInMemory(fields);
+    for i : uint64 := |fields| as uint64 downto 0
       invariant sum == SumValueSize(fields[i..])
     {
       if fields[i].action == ENCRYPT_AND_SIGN {
@@ -174,8 +175,8 @@ module AwsCryptographyDbEncryptionSdkStructuredEncryptionOperations refines Abst
     cmm : CMP.ICryptographicMaterialsManager,
     encryptionContext : Option<CMP.EncryptionContext>,
     algorithmSuiteId: Option<CMP.DBEAlgorithmSuiteId>,
-    encryptedTerminalDataNum : nat,
-    totalEncryptedTerminalValuesSize : nat
+    encryptedTerminalDataNum : uint64,
+    totalEncryptedTerminalValuesSize : uint64
   )
     returns (ret : Result<CMP.EncryptionMaterials, Error>)
     ensures ret.Success? ==>
@@ -216,16 +217,16 @@ module AwsCryptographyDbEncryptionSdkStructuredEncryptionOperations refines Abst
               // - `totalEncryptedTerminalValuesSize` is the sum of the length of all [Terminal Values](./structures.md#terminal-value)
               //   in the [input Structured Data](#structured-data) being encrypted,
               //   as defined by the [input Crypto Schema](#crypto-schema).
-              && var maxLength :=  encryptedTerminalDataNum * 2 + totalEncryptedTerminalValuesSize;
-              && maxLength < INT64_MAX_LIMIT
+              && var maxLength : uint64 :=  Add3(encryptedTerminalDataNum, encryptedTerminalDataNum, totalEncryptedTerminalValuesSize);
+              && maxLength as nat < INT64_MAX_LIMIT
               && (getEncIn.maxPlaintextLength == Some(maxLength as int64))
 
     modifies cmm.Modifies
     requires cmm.ValidState()
     ensures cmm.ValidState()
   {
-    var maxLength :=  encryptedTerminalDataNum * 2 + totalEncryptedTerminalValuesSize;
-    :- Need(maxLength < INT64_MAX_LIMIT, E("Encrypted Size too long."));
+    var maxLength : uint64 :=  Add3(encryptedTerminalDataNum, encryptedTerminalDataNum, totalEncryptedTerminalValuesSize);
+    :- Need(maxLength < INT64_MAX_LIMIT as uint64, E("Encrypted Size too long."));
 
     var algId := GetAlgorithmSuiteId(algorithmSuiteId);
 
@@ -360,8 +361,9 @@ module AwsCryptographyDbEncryptionSdkStructuredEncryptionOperations refines Abst
   method {:vcs_split_on_every_assert} GetV2EncryptionContext2(fields : CryptoList)
     returns (output : Result<CMP.EncryptionContext, Error>)
   {
+    SequenceIsSafeBecauseItIsInMemory(fields);
     var fieldMap : map<ValidUTF8Bytes, Path> := map[];
-    for i := 0 to |fields|
+    for i : uint64 := 0 to |fields| as uint64
     {
       //= specification/structured-encryption/encrypt-path-structure.md#encryption-context-naming
       //# When a key-value pair is added to the encryption context,
@@ -401,10 +403,11 @@ module AwsCryptographyDbEncryptionSdkStructuredEncryptionOperations refines Abst
     //# - 'N' if the attribute was of type Number
     //# - 'L' if the attribute was of type Null or Boolean
     //# - 'B' otherwise
-    for i := 0 to |keys|
+    SequenceIsSafeBecauseItIsInMemory(keys);
+    for i : uint64 := 0 to |keys| as uint64
       invariant forall j | 0 <= j < i :: keys[j] in newContext
       invariant forall k <- newContext :: k in keys[..i]
-      invariant |legend| == |newContext| == i
+      invariant |legend| == |newContext| == i as nat
     {
       assert keys[i] !in newContext by {
         reveal Seq.HasNoDuplicates();
@@ -429,8 +432,9 @@ module AwsCryptographyDbEncryptionSdkStructuredEncryptionOperations refines Abst
         attrStr := attr.value;
       } else if attr.typeId == BOOLEAN {
         legendChar := LEGEND_LITERAL;
-        :- Need(|attr.value| == 1, E("Internal Error : boolean was not of length 1."));
-        attrStr := if attr.value[0] == 0 then FALSE_UTF8 else TRUE_UTF8;
+        SequenceIsSafeBecauseItIsInMemory(attr.value);
+        :- Need(|attr.value| as uint64 == 1, E("Internal Error : boolean was not of length 1."));
+        attrStr := if attr.value[0 as uint32] == 0 then FALSE_UTF8 else TRUE_UTF8;
       } else {
         legendChar := LEGEND_BINARY;
         attrStr := EncodeTerminal(attr);
@@ -619,9 +623,6 @@ module AwsCryptographyDbEncryptionSdkStructuredEncryptionOperations refines Abst
       EncryptStructureOutputHasSinglePaths(cryptoMap, pathOutput.encryptedStructure);
     }
 
-    // This should be provable, but I'm not smart enough
-    :- Need(forall k <- pathOutput.encryptedStructure :: |k.key| == 1, E("Internal Error"));
-
     //= specification/structured-encryption/encrypt-structure.md#behavior
     //= type=implication
     //# The output [Crypto List](encrypt-path-structure.md#crypto-list) produced by [Encrypt Path Structure](encrypt-path-structure.md)
@@ -788,7 +789,8 @@ module AwsCryptographyDbEncryptionSdkStructuredEncryptionOperations refines Abst
     if exists x <- input.plaintextStructure :: x.action == SIGN_AND_INCLUDE_IN_ENCRYPTION_CONTEXT {
       assume {:axiom} input.cmm.Modifies !! {config.materialProviders.History};
       var newEncryptionContext :- GetV2EncryptionContext(input.plaintextStructure);
-      if |newEncryptionContext| != 0 {
+      MapIsSafeBecauseItIsInMemory(newEncryptionContext);
+      if |newEncryptionContext| as uint64 != 0 {
         //= specification/structured-encryption/encrypt-path-structure.md#create-new-encryption-context-and-cmm
         //# An error MUST be returned if any of the entries added to the encryption context in this step
         //# have the same key as any entry already in the encryption context.
@@ -822,8 +824,8 @@ module AwsCryptographyDbEncryptionSdkStructuredEncryptionOperations refines Abst
       cmm,
       Some(encryptionContext),
       input.algorithmSuiteId,
-      CountEncrypted(canonData) as nat,
-      SumValueSize(canonData) as nat);
+      CountEncrypted(canonData),
+      SumValueSize(canonData));
 
     var key : Key := mat.plaintextDataKey.value;
     var alg := mat.algorithmSuite;
@@ -835,7 +837,7 @@ module AwsCryptographyDbEncryptionSdkStructuredEncryptionOperations refines Abst
     //= specification/structured-encryption/encrypt-path-structure.md#calculate-intermediate-encrypted-structured-data
     //# The process used to generate this identifier MUST use a good source of randomness
     //# to make the chance of duplicate identifiers negligible.
-    var randBytes := Random.GenerateBytes(MSGID_LEN as int32);
+    var randBytes := Random.GenerateBytes(MSGID_LEN64 as int32);
     var msgID :- randBytes.MapFailure(e => Error.AwsCryptographyPrimitives(e));
     var head :- Header.Create(input.tableName, canonData, msgID, mat);
     //= specification/structured-encryption/header.md#commit-key
@@ -851,7 +853,8 @@ module AwsCryptographyDbEncryptionSdkStructuredEncryptionOperations refines Abst
     //# The Header Field Value MUST be the full serialized [header](header.md) with commitment.
     var headerAttribute := ValueToData(headerSerialized, BYTES_TYPE_ID);
 
-    :- Need(|canonData| < (UINT32_LIMIT / 3), E("Too many encrypted fields"));
+    SequenceIsSafeBecauseItIsInMemory(canonData);
+    :- Need(|canonData| as uint64 < Crypt.ONE_THIRD_MAX_INT32 as uint64, E("Too many encrypted fields"));
     // input canonData has all input fields, none encrypted
     // output canonData has all input fields, some encrypted
     var encryptedItems : CanonCryptoList :- Crypt.Encrypt(config.primitives, alg, key, head, canonData, input.tableName, input.plaintextStructure);
@@ -892,18 +895,19 @@ module AwsCryptographyDbEncryptionSdkStructuredEncryptionOperations refines Abst
     : string
     requires forall k <- inputFields :: k in inputContext
   {
-    if |inputFields| == 0 then
+    SequenceIsSafeBecauseItIsInMemory(inputFields);
+    if |inputFields| as uint64 == 0 then
       ""
     else
-      var key := inputFields[0];
+      var key := inputFields[0 as uint32];
       if key in headContext && headContext[key] != inputContext[key] then
         var keyStr := SafeDecode(key);
         var headStr := SafeDecode(headContext[key]);
         var inputStr := SafeDecode(inputContext[key]);
         var msg := "input context for " + keyStr + " was " + inputStr + " but stored context had " + headStr + "\n";
-        msg + DescribeMismatch(inputFields[1..], inputContext, headContext)
+        msg + DescribeMismatch(inputFields[1 as uint32..], inputContext, headContext)
       else
-        DescribeMismatch(inputFields[1..], inputContext, headContext)
+        DescribeMismatch(inputFields[1 as uint32..], inputContext, headContext)
   }
 
   function method DetectMismatch(inputContext : CMP.EncryptionContext, headContext : CMP.EncryptionContext)
@@ -911,7 +915,8 @@ module AwsCryptographyDbEncryptionSdkStructuredEncryptionOperations refines Abst
   {
     var inputFields := SortedSets.ComputeSetToOrderedSequence2(inputContext.Keys, ByteLess);
     var str := DescribeMismatch(inputFields, inputContext, headContext);
-    if |str| == 0 then
+    SequenceIsSafeBecauseItIsInMemory(str);
+    if |str| as uint64 == 0 then
       Pass
     else
       Fail(E("Encryption Context Mismatch\n" + str))
@@ -1143,7 +1148,8 @@ module AwsCryptographyDbEncryptionSdkStructuredEncryptionOperations refines Abst
       //# [Terminal Data](./structures.md#terminal-data)
       //# in the input record, plus the Legend.
       var newEncryptionContext :- GetV2EncryptionContext(UnCanon(canonData));
-      if |newEncryptionContext| != 0 {
+      MapIsSafeBecauseItIsInMemory(newEncryptionContext);
+      if |newEncryptionContext| as uint64 != 0 {
         //= specification/structured-encryption/decrypt-path-structure.md#create-new-encryption-context-and-cmm
         //# An error MUST be returned if any of the entries added to the encryption context in this step
         //# have the same key as any entry already in the encryption context.
